coq/Langs/Util.v
@@ -1,0 +1,134 @@
+Set Implicit Arguments.
+Require Import Lists.List.
+
+
+Section Util.
+
+Class HasEquality (A : Type) := eq : A -> A -> bool.
+
+Inductive mapind {A : Type} (H : HasEquality A) (B : Type) : Type :=
+| mapNil : mapind H B
+| mapCons : A -> B -> mapind H B -> mapind H B
+.
+Fixpoint length { A : Type } {H : HasEquality A} {B : Type} (x : mapind H B) : nat :=
+  match x with
+  | mapNil _ _ => 0
+  | mapCons _a _b xs => 1 + (length xs)
+  end
+.
+
+Definition dom { A : Type } {H : HasEquality A} {B : Type} (m : mapind H B) : list A :=
+  let fix dom_aux (m : mapind H B) :=
+    match m with
+    | mapNil _ _ => @List.nil A
+    | mapCons a _b m' => @List.cons A a (dom_aux m')
+    end
+  in dom_aux m
+.
+Definition img { A : Type } {H : HasEquality A} {B : Type} (m : mapind H B) : list B :=
+  let fix img_aux (m : mapind H B) :=
+    match m with
+    | mapNil _ _ => @List.nil B
+    | mapCons _a b m' => @List.cons B b (img_aux m')
+    end
+  in img_aux m
+.
+Definition append { A : Type } {H : HasEquality A} {B : Type} (m0 m1 : mapind H B) : mapind H B :=
+  let fix append_aux (m0 : mapind H B) :=
+    match m0 with
+    | mapNil _ _ => m1
+    | mapCons a b m' => mapCons a b (append_aux m')
+    end
+  in append_aux m0
+.
+(* '↦' is `\mapsto` and '◘' is `\inversebullet`*)
+Notation "a '↦' b '◘' M" := (mapCons a b M) (at level 81, b at next level).
+Notation "M1 '◘' M2" := (append M1 M2) (at level 82, M2 at next level).
+
+Definition splitat { A : Type } {H : HasEquality A} {B : Type} (m : mapind H B) (x : A)
+  : option((mapind H B) * A * B * (mapind H B)) :=
+  let fix doo (accM : mapind H B) (m : mapind H B) :=
+    match m with
+    | mapNil _ _ => None
+    | mapCons a b m' => if eq a x then
+                         Some(accM, a, b, m')
+                       else
+                         doo (a ↦ b ◘ accM) m'
+    end
+  in doo (mapNil H B) m
+.
+
+Definition mget { A : Type } { H : HasEquality A } { B : Type } (m : mapind H B) (x : A) : option B :=
+  let fix doo (m : mapind H B) :=
+    match m with
+    | mapNil _ _=> None
+    | mapCons a b m' => if eq a x then
+                         Some b
+                       else
+                         doo m'
+    end
+  in doo m
+.
+Definition mset { A : Type } { H : HasEquality A } { B : Type } (m : mapind H B) (x : A) (v : B)
+  : option(mapind H B) :=
+  let fix doo (m : mapind H B) :=
+    match m with
+    | mapNil _ _ => None
+    | mapCons a b m'  => if eq a x then
+                          Some(mapCons a v m')
+                        else
+                          match doo m' with
+                          | None => None
+                          | Some m'' => Some(a ↦ b ◘ m'')
+                          end
+    end
+  in doo m
+.
+
+(** These are synthetic. They simply allow us to write e.g. `PrimStep` instead of supplying it with parameters *)
+Class ExprClass (Expr : Type) := {}.
+Class RuntimeExprClass (Expr : Type) := {}.
+Class TraceEvent (Ev : Type) := {}.
+Class ProgClass (A : Type) (Prog : Type) `{ExprClass A} := Cprog__Class : A -> A -> A -> Prog.
+
+(** Since we only care about security properties anyways, it's fine to stay in "traces are lists"-land *)
+Inductive tracepref {Ev : Type} `{TraceEvent Ev} : Type :=
+| Tnil : tracepref
+| Tcons (e : Ev) (As : tracepref) : tracepref
+.
+Fixpoint Tappend {Ev : Type} `{TraceEvent Ev} (As Bs : tracepref) : tracepref :=
+  match As with
+  | Tnil => Bs
+  | Tcons e Cs => Tcons e (Tappend Cs Bs)
+  end
+.
+(* Use this to define a coercion *)
+Definition ev_to_tracepref {Ev : Type} `{TraceEvent Ev} (e : Ev) : tracepref := Tcons e Tnil.
+
+(* Step-Relation typeclasses. Used as a hack for "overloading" notations *)
+Class PrimStep (A : Type) (Ev : Type) `{RuntimeExprClass A} `{TraceEvent Ev} := pstep__Class : A -> Ev -> A -> Prop.
+Class CtxStep (A : Type) (Ev : Type) `{RuntimeExprClass A} `{TraceEvent Ev} := estep__Class : A -> Ev -> A -> Prop.
+Class MultStep (A : Type) (Ev : Type) `{RuntimeExprClass A} `{TraceEvent Ev} := sstep__Class : A -> tracepref -> A -> Prop.
+Class ProgStep (A B : Type) (Ev : Type) (Prog : Type)
+               `{ExprClass A} `{RuntimeExprClass B} `{TraceEvent Ev} `{ProgClass A Prog}
+  := wstep__Class : Prog -> tracepref -> B -> Prop.
+Class VDash (A B C : Type) `{ExprClass B} := vDash : A -> B -> C -> Prop.
+
+End Util.
+
+#[global]
+Notation "a '↦' b '◘' M" := (mapCons a b M) (at level 81, b at next level).
+#[global]
+Notation "M1 '◘' M2" := (append M1 M2) (at level 82, M2 at next level).
+#[global]
+Notation "As '·' Bs" := (Tappend As Bs) (at level 81).
+#[global]
+Notation "e0 '--[' a ']-->' e1" := (pstep__Class e0 a e1) (at level 82, e1 at next level).
+#[global]
+Notation "e0 '==[' a ']==>' e1" := (estep__Class e0 a e1) (at level 82, e1 at next level).
+#[global]
+Notation "e0 '==[' a ']==>*' e1" := (sstep__Class e0 a e1) (at level 82, e1 at next level).
+#[global]
+Notation "'PROG[' e0 '][' ep '][' e1 ']====[' As ']===>' r" := (wstep__Class (Cprog__Class e0 ep e1) As r) (at level 81, r at next level).
+#[global]
+Notation "G '|-' e ':' t" := (vDash G e t) (at level 200, t at next level).
